feat: skeleton for BitVec.add

LeanSAT/Reflect/BVExpr/Basic.lean
@@ -27,6 +27,7 @@ inductive BVBinOp where
 | and
 | or
 | xor
+| add
 
 namespace BVBinOp
 
@@ -34,6 +35,7 @@ def toString : BVBinOp → String
   | and => "&&"
   | or => "||"
   | xor => "^"
+  | add => "+"
 
 instance : ToString BVBinOp := ⟨toString⟩
 
@@ -41,10 +43,12 @@ def eval : BVBinOp → (BitVec w → BitVec w → BitVec w)
   | and => (· &&& ·)
   | or => (· ||| ·)
   | xor => (· ^^^ ·)
+  | add => (· + ·)
 
 @[simp] theorem eval_and : eval .and = ((· &&& ·) : BitVec w → BitVec w → BitVec w) := by rfl
 @[simp] theorem eval_or : eval .or = ((· ||| ·) : BitVec w → BitVec w → BitVec w) := by rfl
 @[simp] theorem eval_xor : eval .xor = ((· ^^^ ·) : BitVec w → BitVec w → BitVec w) := by rfl
+@[simp] theorem eval_add : eval .add = ((· + ·) : BitVec w → BitVec w → BitVec w) := by rfl
 
 end BVBinOp
 
