LeanSAT/Reflect/BVExpr/BitBlast/Lemmas/Add.lean
@@ -1,0 +1,124 @@
+import LeanSAT.Reflect.BVExpr.BitBlast.Lemmas.Basic
+import LeanSAT.Reflect.BVExpr.BitBlast.Impl.Add
+
+open AIG
+
+namespace BVExpr
+namespace bitblast
+namespace blastAdd
+
+@[simp]
+theorem denote_mkFullAdderOut (assign : Assignment) (aig : AIG BVBit) (input : FullAdderInput aig)
+    : ⟦mkFullAdderOut aig input, assign.toAIGAssignment⟧
+        =
+      xor
+        (xor
+           ⟦aig, input.lhs, assign.toAIGAssignment⟧
+           ⟦aig, input.rhs, assign.toAIGAssignment⟧)
+        ⟦aig, input.cin, assign.toAIGAssignment⟧
+    := by
+  simp only [mkFullAdderOut, Ref_cast', denote_mkXorCached, denote_projected_entry, Bool.bne_assoc,
+    Bool.bne_left_inj]
+  rw [LawfulOperator.denote_mem_prefix (f := mkXorCached)]
+
+@[simp]
+theorem denote_mkFullAdderCarry (assign : Assignment) (aig : AIG BVBit) (input : FullAdderInput aig)
+    : ⟦mkFullAdderCarry aig input, assign.toAIGAssignment⟧
+        =
+       or
+         (and
+           (xor
+             ⟦aig, input.lhs, assign.toAIGAssignment⟧
+             ⟦aig, input.rhs, assign.toAIGAssignment⟧)
+           ⟦aig, input.cin, assign.toAIGAssignment⟧)
+         (and
+           ⟦aig, input.lhs, assign.toAIGAssignment⟧
+           ⟦aig, input.rhs, assign.toAIGAssignment⟧)
+    := by
+  simp only [mkFullAdderCarry, Ref_cast', Int.reduceNeg, denote_mkOrCached,
+    LawfulOperator.denote_input_entry, denote_mkAndCached, denote_projected_entry',
+    denote_mkXorCached, denote_projected_entry]
+  -- Without conv mode this timeouts
+  conv =>
+    lhs
+    lhs
+    rhs
+    rw [LawfulOperator.denote_mem_prefix (f := mkXorCached) (h := input.cin.hgate)]
+  conv =>
+    lhs
+    rhs
+    lhs
+    rw [LawfulOperator.denote_mem_prefix (f := mkAndCached)]
+    rw [LawfulOperator.denote_mem_prefix (f := mkXorCached) (h := input.lhs.hgate)]
+  conv =>
+    lhs
+    rhs
+    rhs
+    rw [LawfulOperator.denote_mem_prefix (f := mkAndCached)]
+    rw [LawfulOperator.denote_mem_prefix (f := mkXorCached) (h := input.rhs.hgate)]
+
+-- TODO: additional assumption about cin
+-- Proof idea: show that go always pulls through something that is equiv to BitVec.carry at the
+-- next idx. In particular assuming that the thing it was given was BitVec.carry at the current
+theorem go_eq_eval_getLsb (aig : AIG BVBit) (curr : Nat) (hcurr : curr ≤ w) (cin : Ref aig)
+    (s : AIG.RefStream aig curr) (lhs rhs : AIG.RefStream aig w) (assign : Assignment)
+    (lhsExpr rhsExpr : BVExpr w)
+    (hleft : ∀ (idx : Nat) (hidx : idx < w), ⟦aig, lhs.getRef idx hidx, assign.toAIGAssignment⟧ = (lhsExpr.eval assign).getLsb idx)
+    (hright : ∀ (idx : Nat) (hidx : idx < w), ⟦aig, rhs.getRef idx hidx, assign.toAIGAssignment⟧ = (rhsExpr.eval assign).getLsb idx)
+    (hcin :
+      ⟦aig, cin, assign.toAIGAssignment⟧
+        =
+      BitVec.carry curr (lhsExpr.eval assign) (rhsExpr.eval assign) false
+    )
+  : ∀ (idx : Nat) (hidx1 : idx < w) (hidx2 : curr ≤ idx),
+      ⟦
+        (go aig curr hcurr cin s lhs rhs).aig,
+        (go aig curr hcurr cin s lhs rhs).stream.getRef idx hidx1,
+        assign.toAIGAssignment
+      ⟧
+        =
+      ⟦aig, lhs.getRef idx hidx1, assign.toAIGAssignment⟧.xor
+        (⟦aig, rhs.getRef idx hidx1, assign.toAIGAssignment⟧.xor
+          (BitVec.carry idx (lhsExpr.eval assign) (rhsExpr.eval assign) false)) := by
+  intro idx hidx1 hidx2
+  generalize hgo : go aig curr hcurr cin s lhs rhs = res
+  unfold go at hgo
+  sorry
+
+end blastAdd
+
+theorem blastAdd_eq_eval_getLsb (aig : AIG BVBit) (lhs rhs : BVExpr w) (assign : Assignment)
+      (input : BinaryRefStream aig w)
+      (hleft : ∀ (idx : Nat) (hidx : idx < w), ⟦aig, input.lhs.getRef idx hidx, assign.toAIGAssignment⟧ = (lhs.eval assign).getLsb idx)
+      (hright : ∀ (idx : Nat) (hidx : idx < w), ⟦aig, input.rhs.getRef idx hidx, assign.toAIGAssignment⟧ = (rhs.eval assign).getLsb idx)
+    : ∀ (idx : Nat) (hidx : idx < w),
+        ⟦(blastAdd aig input).aig, (blastAdd aig input).stream.getRef idx hidx, assign.toAIGAssignment⟧
+          =
+        (lhs.eval assign + rhs.eval assign).getLsb idx := by
+  intro idx hidx
+  rw [BitVec.getLsb_add]
+  . rw [← hleft idx hidx]
+    rw [← hright idx hidx]
+    unfold blastAdd
+    dsimp
+    rw [blastAdd.go_eq_eval_getLsb _ 0 (by omega) _ _ _ _ assign lhs rhs _ _]
+    . -- TODO: API lemmas
+      simp [BinaryRefStream.cast]
+      rw [LawfulOperator.denote_mem_prefix (f := mkConstCached)]
+      rw [LawfulOperator.denote_mem_prefix (f := mkConstCached)]
+    . simp
+    . omega
+    . intros
+      -- TODO: API lemmas
+      simp [BinaryRefStream.cast]
+      rw [LawfulOperator.denote_mem_prefix (f := mkConstCached)]
+      rw [hleft]
+    . intros
+      -- TODO: API lemmas
+      simp [BinaryRefStream.cast]
+      rw [LawfulOperator.denote_mem_prefix (f := mkConstCached)]
+      rw [hright]
+  . assumption
+
+end bitblast
+end BVExpr
